additions to support more of bedrock.

src/MultiMem.v
@@ -1,3 +1,4 @@
+Require Import List.
 Require Import Heaps.
 
 Set Implicit Arguments.
@@ -11,6 +12,19 @@ Section parametric.
       | 0 => unit
       | S n => prod T (vector n)
     end.
+
+  Fixpoint to_list (n : nat) : vector n -> list T :=
+    match n as n return vector n -> list T with
+      | 0 => fun _ => nil
+      | S n => fun x => fst x :: to_list _ (snd x)
+    end.
+
+  Definition NoDup_v (n : nat) (v : vector n) : Prop :=
+    NoDup (to_list _ v).
+
+  Definition disjoint_v (n n' : nat) (v : vector n) (v' : vector n') : Prop :=
+    forall x, In x (to_list _ v) -> ~In x (to_list _ v').
+
 End parametric.
 
 Section multi_mem.
@@ -61,6 +75,110 @@ End multi_mem.
 
 Module MultiSepMemFacts (SM : SeparationMemory).
   
+  Require Import Reflection.
+
+  Lemma smem_multi_write_footprint : forall (N : nat) b b' addrs vals,
+    @multi_write_addrs SM.smem SM.M.addr SM.M.value SM.smem_set N addrs vals b = Some b' ->
+    (forall a, ~In a (to_list _ _ addrs) -> SM.smem_get a b = SM.smem_get a b').
+  Proof.
+    induction N; simpl; intros.
+    { inversion H; auto. }
+    { match goal with
+      | [ H : match ?X with _ => _ end = Some _ |- _ ] =>
+        consider X; intros; try congruence
+      end.
+      eapply IHN in H1; eauto.
+      rewrite <- H1.
+      symmetry. eapply SM.smem_set_get_neq; eauto. }
+  Qed.
+
+  Lemma smem_multi_read_footprint : forall T (N : nat) b b' addrs k,
+    (forall a, In a (to_list _ _ addrs) -> SM.smem_get a b = SM.smem_get a b') ->
+    @multi_read_addrs T SM.smem SM.M.addr SM.M.value SM.smem_get b N addrs k = 
+    @multi_read_addrs T SM.smem SM.M.addr SM.M.value SM.smem_get b' N addrs k.
+  Proof.
+    induction N; simpl; intros; auto.
+    { rewrite H; eauto.
+      match goal with
+      | [ |- match ?X with _ => _ end = _ ] =>
+        consider X; intros; try congruence
+      end. eauto. }
+  Qed.
+
+  Lemma smem_read_write_eq_multi' : forall T (N : nat) k b b' addrs vals,
+    NoDup_v _ _ addrs ->
+    @multi_write_addrs SM.smem SM.M.addr SM.M.value SM.smem_set N addrs vals b = Some b' ->
+    @multi_read_addrs T SM.smem SM.M.addr SM.M.value SM.smem_get b' N addrs k = Some (k vals).
+  Proof.
+    induction N; simpl; intros.
+    { inversion H0; destruct vals; intuition auto. }
+    { match goal with
+      | [ H : match ?X with _ => _ end = Some _ |- _ ] =>
+        consider X; intros; try congruence
+      end.
+      inversion H; clear H; subst.
+      match goal with
+        | [ |- match ?X with _ => _ end = Some _ ] =>
+        consider X; intros; try congruence
+      end.
+      { generalize (smem_multi_write_footprint _ _ _ _ H1 (fst addrs) H4). 
+        eapply IHN with (k := fun vs => k (v, vs)) in H1; eauto.
+        generalize (SM.smem_set_get_eq _ _ _ _ H0).
+        intros. rewrite H1. f_equal. f_equal. destruct vals; simpl; f_equal.
+        simpl in *.
+        clear - H H2 H3. unfold vector in *.
+        rewrite H in H3. rewrite H2 in H3. inversion H3; auto. }
+      { exfalso.
+        generalize (smem_multi_write_footprint _ _ _ _ H1 (fst addrs) H4). 
+        eapply IHN with (k := fun vs => k (fst vals,vs)) in H1; eauto.
+        intuition.        
+        generalize (SM.smem_set_get_eq _ _ _ _ H0). unfold vector in *.
+        rewrite H2. rewrite H. congruence. } }
+  Qed.
+
+  Lemma smem_read_write_neq_multi' : forall T (N : nat) k b b' addrs addrs' vals,
+    disjoint_v _ _ _ addrs addrs' ->    
+    @multi_write_addrs SM.smem SM.M.addr SM.M.value SM.smem_set N addrs vals b = Some b' ->
+    @multi_read_addrs T SM.smem SM.M.addr SM.M.value SM.smem_get b' N addrs' k = 
+      @multi_read_addrs T SM.smem SM.M.addr SM.M.value SM.smem_get b N addrs' k.
+  Proof.
+    induction N; simpl; intros.
+    { inversion H0; destruct vals; intuition auto. }
+    { match goal with
+      | [ H : match ?X with _ => _ end = Some _ |- _ ] =>
+        consider X; intros; try congruence
+      end.
+      match goal with
+        | [ |- match ?X with _ => _ end = _ ] =>
+        consider X; intros; try congruence
+      end.
+      { generalize (smem_multi_write_footprint _ _ _ _ H1); intro.
+        eapply IHN with (addrs' := snd addrs') (k := fun vs => k (v, vs)) in H1; eauto.
+        { match goal with
+          | [ |- _ = match ?X with _ => _ end ] =>
+            replace X with (Some v)
+          end.
+          etransitivity. eapply H1.
+          eapply smem_multi_read_footprint.
+          { intros.
+            eapply (SM.smem_set_get_neq _ _ _ _ H0 a).
+            red in H. simpl in H. intro.
+            eapply H; eauto. }
+          { rewrite <- H3 in H2.
+            generalize (SM.smem_set_get_neq _ _ _ _ H0 (fst addrs')).
+            rewrite <- H2. intro. apply H4. 
+            intro. eapply H. left. reflexivity.
+            exfalso. eapply H. left. reflexivity. left; auto.
+            intro. eapply H. right. eapply H4. left. auto. } }
+        { red; intros. intro. eapply H.
+          right; eassumption. right; eassumption. } }
+      { generalize (smem_multi_write_footprint _ _ _ _ H1).
+        eapply SM.smem_set_get_neq in H0. rewrite <- H0.
+        intro. rewrite H3. rewrite H2; auto.
+        { intro. eapply H. right; eapply H4. left; reflexivity. }
+        { intro. eapply H. left; reflexivity. left. auto. } } }
+  Qed.
+
   Lemma split_smem_read_multi' : forall T (N : nat) k a b c addrs v,
     SM.split a b c ->
       @multi_read_addrs T SM.smem SM.M.addr SM.M.value SM.smem_get b N addrs k = Some v ->
@@ -100,6 +218,28 @@ Module MultiSepMemFacts (SM : SeparationMemory).
     Variable footprint : SM.M.addr -> vector SM.M.addr N.
     Variable implode : vector SM.M.value N -> T.
     Variable explode : T -> vector SM.M.value N.
+
+    Theorem split_multi_read_write_eq : forall b b' p v,
+      implode (explode v) = v ->
+      NoDup_v _ _ (footprint p) ->
+      @multi_write T SM.smem SM.M.addr SM.M.value N footprint explode SM.smem_set p v b = Some b' ->
+      @multi_read T SM.smem SM.M.addr SM.M.value N footprint implode SM.smem_get p b' = Some v.
+    Proof.
+      unfold multi_read, multi_write; intros.
+      eapply smem_read_write_eq_multi' with (k := implode) in H1; eauto. intuition.
+      rewrite H1. rewrite H; auto.
+    Qed.
+
+    Theorem split_multi_read_write_neq : forall b b' p p' v,
+      implode (explode v) = v ->
+      disjoint_v _ _ _ (footprint p) (footprint p') ->
+      @multi_write T SM.smem SM.M.addr SM.M.value N footprint explode SM.smem_set p v b = Some b' ->
+      @multi_read T SM.smem SM.M.addr SM.M.value N footprint implode SM.smem_get p' b' = 
+      @multi_read T SM.smem SM.M.addr SM.M.value N footprint implode SM.smem_get p' b. 
+    Proof.
+      unfold multi_read, multi_write; intros.
+      eapply smem_read_write_neq_multi' with (k := implode) in H1; eauto. 
+    Qed.
 
     Theorem split_multi_read : forall a b c p v,
       SM.split a b c ->
